\documentclass[12pt]{article}
\setlength{\parindent}{0pt}
\usepackage{amsmath}
\begin{document}
Compute the following:
\newline
x = $\sum\limits^{\infty }_{n=1 }\frac{1}{2\textsuperscript{n }}$=
\newline
x = $\sum\limits^{\infty }_{n=1 }\frac{1}{n }$=
\newline
x = $\sum\limits^{\infty }_{n=0 }\frac{(3 + 2n)}{2\textsuperscript{n }}$=
\newline
x = $\sum\limits^{\infty }_{n=1 }\frac{(-1)\textsuperscript{n-1}}{n }$=
\newline
x = $\sum\limits^{\infty }_{n=1 }\frac{csc\textsuperscript{2}n}{n\textsuperscript{3 }}$=
\end{document}